draft for expression evaluator

examples/tactics/Imp.fst
@@ -1,15 +1,160 @@
 module Imp
 
-open FStar.Tactics
+#set-options "--debug Imp --debug_level SMTQuery"
 
-(* Testing that intro works on implicits seamlessly *)
+open FStar.Mul
 
-let tau () : Tac unit =
-    let b = intro () in
-    exact (pack (Tv_Var (bv_of_binder b)))
+type rval = int
+type reg = | R of n:nat{n < 10}
+type regmap = reg -> rval
 
-let f :    int -> int = synth_by_tactic tau
-let g : #x:int -> int = synth_by_tactic tau
+noeq
+type inst =
+    | Add : reg -> reg -> reg -> inst
+    | Sub : reg -> reg -> reg -> inst
+    | Mul : reg -> reg -> reg -> inst
+    | Const : rval -> reg -> inst
 
-let _ = assert (f  3 == 3)
-let _ = assert (g #3 == 3)
+type prog = list inst
+
+val override : reg -> rval -> regmap -> regmap
+let override r v rm =
+    fun r' ->
+        if r = r'
+        then v
+        else rm r'
+
+val step : inst -> regmap -> regmap
+let step i rm =
+    match i with
+    | Add r1 r2 r3 -> override r3 (rm r1 + rm r2) rm
+    | Sub r1 r2 r3 -> override r3 (rm r1 - rm r2) rm
+    | Mul r1 r2 r3 -> override r3 (rm r1 * rm r2) rm
+    | Const v r    -> override r v rm
+
+val run : prog -> regmap -> regmap
+let run prog rm = List.Tot.fold_left (fun rm i -> step i rm) rm prog
+
+(* Run in all zeros and get the 0th reg *)
+val eval : prog -> rval
+let eval p = let rm = run p (fun _ -> 0) in rm (R 0)
+
+let equiv p1 p2 = eval p1 == eval p2
+
+let mk42 : prog = [
+    Const 1 (R 0);
+    Add (R 0) (R 0) (R 1);
+    Add (R 1) (R 1) (R 0);
+    Add (R 0) (R 0) (R 1);
+    Add (R 1) (R 1) (R 0);
+    Add (R 0) (R 0) (R 1);
+    Add (R 1) (R 0) (R 0);
+    Const 6 (R 1);
+    Sub (R 0) (R 1) (R 0);
+]
+
+let _ = assert_norm (eval mk42 == 42)
+
+let add1 x y : prog = [
+    Const x (R 0);
+    Const y (R 1);
+    Add (R 0) (R 1) (R 0);
+]
+    
+let add2 x y : prog = [
+    Const y (R 1);
+    Const x (R 0);
+    Add (R 0) (R 1) (R 0);
+]
+    
+let add3 x y : prog = [
+    Const x (R 0);
+    Const y (R 1);
+    Add (R 1) (R 0) (R 0);
+]
+    
+let add4 x y : prog = [
+    Const y (R 1);
+    Const x (R 0);
+    Add (R 1) (R 0) (R 0);
+]
+
+(* All of these identies are quite easy by normalization. Once we fix
+ * #1482, they will not even require SMT. *)
+let _ = assert_norm (forall x y. equiv (add1 x y) (add2 x y))
+let _ = assert_norm (forall x y. equiv (add1 x y) (add3 x y))
+let _ = assert_norm (forall x y. equiv (add1 x y) (add4 x y))
+let _ = assert_norm (forall x y. equiv (add2 x y) (add3 x y))
+let _ = assert_norm (forall x y. equiv (add2 x y) (add4 x y))
+let _ = assert_norm (forall x y. equiv (add3 x y) (add4 x y))
+
+(* Without normalizing, they require fuel, or else fail *)
+#push-options "--max_fuel 0"
+[@fail] let _ = assert (forall x y. equiv (add1 x y) (add2 x y))
+[@fail] let _ = assert (forall x y. equiv (add1 x y) (add3 x y))
+[@fail] let _ = assert (forall x y. equiv (add1 x y) (add4 x y))
+[@fail] let _ = assert (forall x y. equiv (add2 x y) (add3 x y))
+[@fail] let _ = assert (forall x y. equiv (add2 x y) (add4 x y))
+[@fail] let _ = assert (forall x y. equiv (add3 x y) (add4 x y))
+#pop-options
+
+(* poly5 x = x^5 + x^4 + x^3 + x^2 + x^1 + 1 *)
+
+let poly5 x : prog = [
+    Const 1 (R 0);
+    Const x (R 1);
+    Mul (R 1) (R 1) (R 2);
+    Mul (R 1) (R 2) (R 3);
+    Mul (R 1) (R 3) (R 4);
+    Mul (R 1) (R 4) (R 5);
+    Add (R 0) (R 1) (R 0);
+    Add (R 0) (R 2) (R 0);
+    Add (R 0) (R 3) (R 0);
+    Add (R 0) (R 4) (R 0);
+    Add (R 0) (R 5) (R 0);
+]
+
+let _ = assert_norm (eval (poly5 1) == 6)
+let _ = assert_norm (eval (poly5 2) == 63)
+let _ = assert_norm (eval (poly5 3) == 3*3*3*3*3 + 3*3*3*3 + 3*3*3 + 3*3 + 3 + 1)
+
+(* Bunch of fuel to even prove ground facts *)
+#push-options "--max_fuel 12"
+let _ = assert (eval (poly5 1) == 6)
+let _ = assert (eval (poly5 2) == 63)
+let _ = assert (eval (poly5 3) == 3*3*3*3*3 + 3*3*3*3 + 3*3*3 + 3*3 + 3 + 1)
+#pop-options
+
+(* A different way of computing it *)
+let poly5' x : prog = [
+    Const 1 (R 0);
+    Const x (R 1);
+    Const 1 (R 2);
+    Mul (R 0) (R 1) (R 0);
+    Add (R 0) (R 2) (R 0);
+    Mul (R 0) (R 1) (R 0);
+    Add (R 0) (R 2) (R 0);
+    Mul (R 0) (R 1) (R 0);
+    Add (R 0) (R 2) (R 0);
+    Mul (R 0) (R 1) (R 0);
+    Add (R 0) (R 2) (R 0);
+    Mul (R 0) (R 1) (R 0);
+    Add (R 0) (R 2) (R 0);
+]
+
+(* Seems to do the same *)
+let _ = assert_norm (eval (poly5' 1) == 6)
+let _ = assert_norm (eval (poly5' 2) == 63)
+let _ = assert_norm (eval (poly5' 3) == 3*3*3*3*3 + 3*3*3*3 + 3*3*3 + 3*3 + 3 + 1)
+
+(* Same *)
+#push-options "--max_fuel 14"
+let _ = assert (eval (poly5' 1) == 6)
+let _ = assert (eval (poly5' 2) == 63)
+let _ = assert (eval (poly5' 3) == 3*3*3*3*3 + 3*3*3*3 + 3*3*3 + 3*3 + 3 + 1)
+#pop-options
+
+[@fail]
+let _ = assert (forall x. poly5 x `equiv` poly5' x)
+
+let _ = assert_norm (forall x. poly5 x `equiv` poly5' x)
